Soundness.v
@@ -6,6 +6,14 @@ Require Import Typing.
 Require Import Constraint.
 Require Import TypeSubst.
 
+Lemma apply_solution: forall tsubst tenv T S1 S2 U1 U2 t1 t2 C C1 C2,
+  Constraint.Solution tsubst T tenv (Apply t1 t2) S2 C ->
+  TypeSubst S1 U1 tsubst ->
+  TypeSubst S2 U2 tsubst ->
+  Unified C1 tsubst -> Unified C2 tsubst ->
+  Constraint.Solution tsubst U1 tenv t1 S1 C1 /\
+  Constraint.Solution tsubst U2 tenv t2 S2 C2.
+
 Lemma lambda_solution: forall tsubst T S T1 T2 tenv x t C,
   Constraint.Solution tsubst T tenv (Lambda x T1 t) (FunT T1 T2) C ->
   TypeSubst T2 S tsubst ->
@@ -13,6 +21,7 @@ Lemma lambda_solution: forall tsubst T S T1 T2 tenv x t C,
 Proof.
 unfold Constraint.Solution in |- *.
 intros.
+specialize (H X).
 inversion H.
 split.
  inversion H1.
@@ -61,7 +70,7 @@ intro.
 generalize T.
 pattern t, tenv, S, (nil:tvars), C in |- *.
 apply TypeConstraint_ind.
- intros.
+ (* var *)
  unfold Solution in |- *.
  intros.
  apply
@@ -75,13 +84,16 @@ apply TypeConstraint_ind.
   trivial.
 
   unfold Constraint.Solution in H1.
+  specialize (H1 nil).
   inversion H1.
   inversion H5.
   trivial.
 
+ (* lambda *)
  intros.
  generalize H2; intro.
  unfold Constraint.Solution in H3.
+ specialize (H3 X).
  inversion H3.
  inversion H5.
  inversion H7.
@@ -95,5 +107,23 @@ apply TypeConstraint_ind.
 
   trivial.
 
-(* eapply lambda_solution in H2.
-  apply H1 in H2.*)
+  (* bool *)
+ unfold Solution in |- *.
+ unfold Constraint.Solution in |- *.
+ intros.
+ specialize (H0 nil).
+ inversion H0.
+ inversion H4.
+ inversion H6.
+ apply
+  subst_preserve
+   with (tsubst := tsubst) (t := Bool b) (tenv1 := tenv0) (T := BoolT).
+  apply TBool.
+
+  trivial.
+
+  trivial.
+
+  apply SBoolT.
+
+
